# Quadratic Formula's proof

Have you ever wondered why the quadratic formula is like that?

In this page, you will learn how to prove quadratic formula and also why it is in that form.

$$
x=\frac{-b\pm\sqrt{b^2-4ac}}{2a}
$$

*The quadratic formula*


!!! Warning
    To prove the quadratic equation, we are going to use completion of the square method. Since this method is probably the easiest and most intitive way of proving, we recommend learning how this method before continuing to read this article.
    <iframe width="950" height="534" src="https://www.youtube.com/embed/2MKigAgPZMQ" title="Solving Quadratic Equations By Completing The Square" frameborder="0" allow="accelerometer; autoplay; clipboard-write; encrypted-media; gyroscope; picture-in-picture; web-share" referrerpolicy="strict-origin-when-cross-origin" allowfullscreen></iframe>

## Step 1:
Factor out `a`.

$$
a(x^2+\frac{b}{a})+c=0
$$

## Step 2:
Apply the completion of square. Insert (b/2a)^2 to do this.

$$
a(x^2+\frac{b}{a}+(\frac{b}{2a})^2)-(\frac{b}{2a})^2+c=0
$$

## Step 3:
Simplify.

$$
a(x^2+\frac{b}{a}+\frac{b^2}{4a^2})=\frac{b^2}{4a^2}-c
$$

## Step 4:
Factor.

$$
a(x+\frac{b}{2a})^2=\frac{b^2}{4a^2}-c
$$

## Step 5:
Divide both sides by a.

$$
(x+\frac{b}{2a})^2=\frac{b^2}{4a^2}-\frac{c}{a}
$$

## Step 6:
Simplify the right side.

$$
(x+\frac{b}{2a})^2=\frac{b^2-4ac}{4a^2}
$$

## Step 7:
Take the square root of both sides.

$$
x+\frac{b}{2a}=\pm\sqrt{\frac{b^2-4c}{4a^2}}=\pm\frac{\sqrt{b^2-4ac}}{2a}
$$

!!! Info
    This is where it leaves us with discriminant. â€»The numerator.

## Step 8:
We are almost done!!

The last step is to move the b/2a term.

$$
x=\frac{\pm\sqrt{b^2-4ac}}{2a}-\frac{b}{2a}=\frac{-b\pm\sqrt{b^2-4ac}}{2a}
$$

And this is the complete proof to the quadratic formula!!

If you have time, try using pencil and paper to figure this out again on your own.

